processor/integration/system.v
@@ -134,12 +134,11 @@ module system(
 	  : (mem_rq_addr == 32'h1002404c && !mem_rq_iswrite) ? {(!spi_tx_rdy), 23'h0, spi_rx_buf}
 	  : 32'hxxxxxxxx;
   always @(posedge clk) begin
-    $display(clk);
     if (en_obtain_rq_get && mem_rq_iswrite && mem_rq_addr == 32'h1001200c) begin
       led <= mem_rq_data[23:16];
     end
   end
-  wire spi_tx_en = en_obtain_rq_get && mem_rq_iswrite && mem_rq_addr == 32'h1001200c;
+  wire spi_tx_en = en_obtain_rq_get && mem_rq_iswrite && mem_rq_addr == 32'h10024048;
   reg [3:0] spi_tx_remaining = 0;
   reg [7:0] spi_tx_buf;
   reg [7:0] spi_rx_buf;
@@ -158,41 +157,14 @@ module system(
       spi_tx_remaining <= spi_tx_remaining - 1;
     end
   end
-
 `ifndef SYNTHESIS
   always #1 clk = !clk;
   initial begin
     $dumpfile("system.vcd");
-    $dumpvars(1, mkTop.proc_m9_pinit, mkTop.proc_m9_pc,
-
-    mkTop.CAN_FIRE_RL_proc_m12_reqLd,
-    mkTop.CAN_FIRE_RL_proc_m12_reqSt,
-    mkTop.CAN_FIRE_RL_proc_m12_wbNm,
-    mkTop.CAN_FIRE_RL_proc_m12_wbNmZ,
-    mkTop.WILL_FIRE_RL_proc_m10_decodeLd,
-    mkTop.WILL_FIRE_RL_proc_m10_decodeNm,
-    mkTop.WILL_FIRE_RL_proc_m10_decodeSt,
-    mkTop.WILL_FIRE_RL_proc_m11_execBypass,
-    mkTop.WILL_FIRE_RL_proc_m11_execNm,
-    mkTop.WILL_FIRE_RL_proc_m12_repLd,
-    mkTop.WILL_FIRE_RL_proc_m12_repSt,
-    mkTop.WILL_FIRE_RL_proc_m12_reqLd,
-    mkTop.WILL_FIRE_RL_proc_m12_reqLdZ,
-    mkTop.WILL_FIRE_RL_proc_m12_reqSt,
-    mkTop.WILL_FIRE_RL_proc_m12_wbNm,
-    mkTop.WILL_FIRE_RL_proc_m12_wbNmZ,
-    mkTop.WILL_FIRE_RL_proc_m12_wrongEpoch,
-    mkTop.WILL_FIRE_RL_proc_m9_instFetchRq,
-    mkTop.WILL_FIRE_RL_proc_m9_instFetchRs,
-    mkTop.WILL_FIRE_RL_proc_m9_modifyPc,
-    mkTop.WILL_FIRE_RL_proc_m9_pgmInitAck,
-    mkTop.WILL_FIRE_RL_proc_m9_pgmInitAckEnd,
-    mkTop.WILL_FIRE_RL_proc_m9_pgmInitRq,
-    mkTop.WILL_FIRE_RL_proc_m9_pgmInitRqEnd,
-    mkTop.WILL_FIRE_RL_proc_m9_pgmInitRs,
+    $dumpvars(1, mkTop.proc_m8_pc,
     led, spi_clk, spi_cs, spi_mosi, spi_miso, clk, resetn,
-      rdy_obtain_rq_get, en_obtain_rq_get, mem_rq_iswrite, mem_rq_addr, mem_rq_data, rdy_send_rs_put, ram_rs_en, instant_rs_en, ram_read, spi_tx_buf, spi_rx_buf);
-    #10000 $finish();
+      rdy_obtain_rq_get, en_obtain_rq_get, mem_rq_iswrite, mem_rq_addr, mem_rq_data, rdy_send_rs_put, ram_rs_en, ram_read, instant_rs_en, instant_rs, spi_tx_buf, spi_rx_buf, spi_tx_rdy);
+    #4000 $finish();
   end
 `endif
 endmodule
